@@ -3410,7 +3410,7 @@ Proof.
     (cbn;
     case_decide as Hl'; cbn;
     [rewrite lengthN_correct_rev; f_equal; lia|];
-    unfold list_index;
+    rewrite list_index_eq_find;
     destruct (list_find _ _) as [[n ?]|]; done).
 Qed.
 
